split files

crypto_examples/ntt.dfy
@@ -1,5 +1,6 @@
 include "pow2.dfy"
 include "omega.dfy"
+include "ntt_rec.dfy"
 
 module ntt {
     import opened Seq
@@ -8,397 +9,10 @@ module ntt {
     import opened Mul
     import opened pows_of_2
     import opened omegas
-
-    function {:opaque} poly_eval(a: seq<elem>, x: elem): elem
-    {
-        if |a| == 0 then 0
-        else modadd(First(a), modmul(poly_eval(DropFirst(a), x), x))
-    }
-
-    function method odd_indexed_terms(a: seq<elem>, len: pow2_t): seq<elem>
-        requires |a| == len.full * 2;
-    {
-        seq(len.full, n requires 0 <= n < len.full => a[n * 2 + 1])
-    }
-
-    function method even_indexed_terms(a: seq<elem>, len: pow2_t): seq<elem>
-        requires |a| == len.full * 2;
-    {
-        seq(len.full, n requires 0 <= n < len.full => a[n * 2])
-    }
-
-    lemma poly_eval_base_lemma(a: seq<elem>, x: elem)
-        requires |a| == 1;
-        ensures poly_eval(a, x) == a[0];
-    {
-        reveal poly_eval();
-    }
-
-    lemma {:axiom} poly_eval_split_lemma(a: seq<elem>, 
-        a_e: seq<elem>, a_o: seq<elem>, len: pow2_t, x: elem)
-        requires |a| == len.full * 2;
-        requires a_e == even_indexed_terms(a, len)
-        requires a_o == odd_indexed_terms(a, len)
-        ensures var sqr := modmul(x, x);
-            poly_eval(a, x)
-                == 
-            modadd(poly_eval(a_e, sqr), modmul(x, poly_eval(a_o, sqr)));
-        decreases |a|;
-    // {
-    //     pow2_basics(len);
-
-    //     if |a| == 2 {
-    //         assert a_e == [a[0]];
-    //         assert a_o == [a[1]];
-
-    //         var sqr := modmul(x, x);
-
-    //         calc == {
-    //             poly_eval(a, x);
-    //             {
-    //                 reveal poly_eval();
-    //                 assert DropFirst(a) == a_o;
-    //             }
-    //             modadd(a[0], modmul(poly_eval(a_o, x), x));
-    //             {
-    //                 poly_eval_base_lemma(a_o, x);
-    //                 assert poly_eval(a_o, x) == a[1];
-    //             }
-    //             modadd(a[0], modmul(a[1], x));
-    //             {
-    //                 poly_eval_base_lemma(a_e, sqr);
-    //                 assert poly_eval(a_e, sqr) == a[0];
-    //             }
-    //             modadd(poly_eval(a_e, sqr), modmul(a[1], x));
-    //             {
-    //                 poly_eval_base_lemma(a_o, sqr);
-    //                 assert poly_eval(a_o, sqr) == a[1];
-    //             }
-    //             modadd(poly_eval(a_e, sqr), modmul(x, poly_eval(a_o, sqr)));
-    //         }
-    //         return;
-    //     }
-
-    //     var len' := pow2_half(len);
-    //     var a_ee := even_indexed_terms(a_e, len');
-    //     var a_eo := odd_indexed_terms(a_e, len');
-    //     var a_oe := even_indexed_terms(a_o, len');
-    //     var a_oo := odd_indexed_terms(a_o, len');
-
-    //     calc == {
-    //         poly_eval(a, x);
-    //         {
-    //             reveal poly_eval();
-    //             assert DropFirst(a) == a_o;
-    //         }
-    //         modadd(a[0], modmul(poly_eval(a_o, x), x));
-    //     }
-
-    //     assume false;
-    // }
-
-    predicate poly_eval_all_points(a: seq<elem>, y: seq<elem>, len: pow2_t)
-        requires 0 <= len.exp <= L
-    {
-        && |y| == |a| == len.full
-        && (forall i: nat :: i < len.full ==>
-            y[i] == poly_eval(a, omega_nk(len, i)))
-    }
-
-    lemma y_k_value(a: seq<elem>,
-        a_e: seq<elem>, a_o: seq<elem>,
-        len': pow2_t, len: pow2_t,
-        omg: elem, k: nat,
-        y_e_k: elem, y_o_k: elem, y_k: elem)
-
-        requires |a| == len'.full * 2;
-        requires 1 <= len.exp <= L;
-        requires len'.exp <= L 
-        requires len' == pow2_half(len);
-        requires k < len'.full;
-        requires a_e == even_indexed_terms(a, len');
-        requires a_o == odd_indexed_terms(a, len');
-
-        requires omg == modpow(omega_n(len), k);
-        requires y_e_k == poly_eval(a_e, omega_nk(len', k));
-        requires y_o_k == poly_eval(a_o, omega_nk(len', k));
-        requires y_k == modadd(y_e_k, modmul(omg, y_o_k));
-        
-        ensures y_k == poly_eval(a, omega_nk(len, k));
-    {
-        var x := omega_nk(len, k);
-        var sqr := modmul(x, x);
-
-        calc == {
-            sqr;
-            {
-                omega_nk_square(len, k);
-            }
-            omega_nk(len, 2 * k);
-            {
-                ntt_cancellation_lemma(len, k);
-            }
-            omega_nk(len', k);
-        }
-
-        calc == {
-            poly_eval(a, x);
-            {
-                poly_eval_split_lemma(a, a_e, a_o, len', x);
-            }
-            modadd(poly_eval(a_e, sqr), modmul(x, poly_eval(a_o, sqr)));
-            {
-                assert poly_eval(a_e, sqr) == y_e_k;
-                assert poly_eval(a_o, sqr) == y_o_k;
-            }
-            modadd(y_e_k, modmul(x, y_o_k));
-            y_k;
-        }
-    }
-
-    lemma y_k'_value(a: seq<elem>,
-        a_e: seq<elem>, a_o: seq<elem>,
-        len': pow2_t, len: pow2_t,
-        omg: elem, k: nat,
-        y_e_k: elem, y_o_k: elem, y_k': elem)
-
-        requires |a| == len'.full * 2;
-        requires 1 <= len.exp <= L;
-        requires len'.exp <= L 
-        requires len' == pow2_half(len);
-        requires k < len'.full;
-        requires a_e == even_indexed_terms(a, len');
-        requires a_o == odd_indexed_terms(a, len');
-
-        requires omg == omega_nk(len, k);
-        requires y_e_k == poly_eval(a_e, omega_nk(len', k));
-        requires y_o_k == poly_eval(a_o, omega_nk(len', k));
-        requires y_k' == modsub(y_e_k, modmul(omg, y_o_k));
-
-        ensures y_k' == poly_eval(a, omega_nk(len, k + len'.full));
-    {
-        var x := omega_nk(len, k + len'.full);
-        var sqr := modmul(x, x);
-
-        calc == {
-            sqr;
-            {
-                omega_nk_square(len, k + len'.full);
-            }
-            omega_nk(len, 2 * k + len.full);
-            {
-                ntt_halving_lemma(len, k);
-            }
-            omega_nk(len, 2 * k);
-            {
-                ntt_cancellation_lemma(len, k);
-            }
-            omega_nk(len', k);
-        }
-
-        calc {
-            x;
-            omega_nk(len, k + len'.full);
-            {
-                omega_nk_mul_lemma(len, k, len'.full);
-            }
-            modmul(omg, omega_nk(len, len'.full));
-            {
-                ntt_neg_one_lemma(len);
-            }
-            modmul(omg, Q - 1);
-            (omg * (Q - 1)) % Q;
-            {
-                LemmaMulIsDistributiveSubAuto();
-            }
-            (omg * Q - omg) % Q;
-            {
-                LemmaModMultiplesVanishAuto();
-            }
-            (- (omg as int)) % Q;
-        }
-
-        calc == {
-            poly_eval(a, x);
-            {
-                poly_eval_split_lemma(a, a_e, a_o, len', x);
-            }
-            modadd(poly_eval(a_e, sqr), modmul(x, poly_eval(a_o, sqr)));
-            {
-                assert poly_eval(a_e, sqr) == y_e_k;
-                assert poly_eval(a_o, sqr) == y_o_k;
-            }
-            modadd(y_e_k, modmul(x, y_o_k));
-            (y_e_k + (x * y_o_k) % Q) % Q;
-            {
-                LemmaAddModNoopRight(y_e_k, x * y_o_k, Q);
-            }
-            (y_e_k + x * y_o_k) % Q;
-            (y_e_k + (- (omg as int) % Q) * y_o_k ) % Q;
-            (y_e_k + (- (omg as int) % Q) * (y_o_k % Q)) % Q;
-            {
-                LemmaMulModNoopLeft(- (omg as int), y_o_k, Q);
-            }
-            (y_e_k + ((-(omg as int) * y_o_k) % Q)) % Q;
-            {
-                LemmaAddModNoopRight(y_e_k, -(omg as int) * y_o_k, Q);
-            }
-            (y_e_k + (-(omg as int) * y_o_k)) % Q;
-            (y_e_k + ((-1 * (omg as int)) * y_o_k)) % Q;
-            {
-                LemmaMulIsAssociativeAuto();
-            }
-            (y_e_k - 1 * (omg as int) * y_o_k) % Q;
-            {
-                LemmaMulBasicsAuto();
-            }
-            (y_e_k - (omg as int) * y_o_k) % Q;
-            (y_e_k - (omg * y_o_k)) % Q;
-            {
-                LemmaSubModNoopRight(y_e_k, omg * y_o_k, Q);
-            }
-            (y_e_k - (omg * y_o_k) % Q) % Q;
-            modsub(y_e_k, modmul(omg, y_o_k));
-            y_k';
-        }
-    }
-
-    lemma omg_inv(omgn: elem, omg: elem, len: pow2_t, k: nat)
-        requires len.exp <= L
-        requires omgn == omega_n(len);
-        requires omg == modpow(omgn, k);
-        ensures modmul(omg, omgn) == modpow(omgn, k+1);
-    {
-        var omg' := modmul(omg, omgn);
-        calc == {
-            omg';
-            modmul(omg, omgn);
-            modmul(modpow(omgn, k), omgn);
-            (Pow(omgn, k) % Q * omgn) % Q;
-            {
-                LemmaMulModNoopLeft(Pow(omgn, k), omgn, Q);
-            }
-            (Pow(omgn, k) * omgn) % Q;
-            {
-                LemmaPow1(omgn);
-                assert omgn == Pow(omgn, 1);
-                LemmaPowAdds(omgn, k, 1);
-            }
-            Pow(omgn, k+1) % Q;
-            modpow(omgn, k+1);
-        }
-    }
-
-    lemma ntt_base_case(a: seq<elem>, len: pow2_t)
-        requires len.full == 1;
-        requires |a| == len.full;
-        ensures len.exp == 0;
-        ensures a[0] == poly_eval(a, omega_nk(len, 0));
-    {
-        pow2_basics(len);
-        assert len.exp == 0;
-
-        calc {
-            poly_eval(a, omega_nk(len, 0));
-            {
-                omega_nk_canonical(len, 0);
-                assert omega_nk(len, 0) == 
-                    Pow(G, Pow2(L - len.exp) * 0) % Q;
-            }
-            poly_eval(a, Pow(G, Pow2(L - len.exp) * 0) % Q);
-            poly_eval(a, Pow(G, 0) % Q);
-            {
-                LemmaPow0(G);
-            }
-            poly_eval(a, 1);
-            {
-                poly_eval_base_lemma(a, 1);
-            }
-            a[0];
-        }
-
-    }
-
-    method ntt_rec(a: seq<elem>, len: pow2_t) returns (y: seq<elem>)
-        requires 1 <= len.full;
-        requires len.exp <= L;
-        requires |a| == len.full;
-        ensures poly_eval_all_points(a, y, len)
-        decreases len.full
-    {
-        if len.full == 1 {
-            ntt_base_case(a, len);
-            return a;
-        }
-
-        var len' := pow2_half(len);
-        var a_e := even_indexed_terms(a, len');
-        var a_o := odd_indexed_terms(a, len');
-
-        var y_e := ntt_rec(a_e, len');
-        var y_o := ntt_rec(a_o, len');
-
-        y := seq(len.full, n requires 0 <= n < len.full => 0);
-
-        var omgn := omega_n(len);
-        var omg := 1;
-        var k := 0;
-
-        assert omg == modpow(omgn, 0) by {
-            LemmaPow0Auto();
-        }
-
-        while (k < len'.full)
-            invariant k <= len'.full;
-            invariant |y| == len.full;
-            invariant len.full == len'.full * 2;
-
-            invariant omg == modpow(omgn, k);
-            invariant forall i: nat :: i < k ==> (
-                && y[i] == poly_eval(a, omega_nk(len, i))
-                && y[i + len'.full] == poly_eval(a, omega_nk(len, i + len'.full)))
-            
-            decreases len'.full - k;
-        {
-            var y_e_k := y_e[k];
-            var y_o_k := y_o[k];
-
-            assert y_e_k == poly_eval(a_e, omega_nk(len', k));
-            assert y_o_k == poly_eval(a_o, omega_nk(len', k));
-
-            var y_k := modadd(y_e_k, modmul(omg, y_o_k));
-            y := y[k := y_k];
-
-            var y_k' := modsub(y_e_k, modmul(omg, y_o_k));
-            y := y[k + len'.full := y_k'];
-
-            y_k_value(a, a_e, a_o, len', len, 
-                omg, k, y_e_k, y_o_k, y_k);
-
-            y_k'_value(a, a_e, a_o, len', len, 
-                omg, k, y_e_k, y_o_k, y_k');
-
-            omg_inv(omgn, omg, len, k);
-            omg := modmul(omg, omgn);
-
-            k := k + 1;
-        }
-
-        forall i: nat
-            ensures i < len.full ==> y[i] == poly_eval(a, omega_nk(len, i))
-        {
-            if i < len'.full {
-                assert y[i] == poly_eval(a, omega_nk(len, i));
-            } else if i < len.full {
-                var j := i - len'.full;
-                assert y[j + len'.full] ==
-                    poly_eval(a, omega_nk(len, j + len'.full));
-            }
-        }
-    }
+    import opened ntt_rec
 
     lemma index_bounded_lemma(
-        index: nat, j: nat, s: nat, k: nat, ki: nat,
+        j: nat, k: nat, ki: nat,
         m: pow2_t, step_count: pow2_t)
         requires m.full >= 2;
         requires 0 <= j < m.full / 2;
@@ -406,16 +20,14 @@ module ntt {
         requires 1 <= m.exp <= L;
         requires step_count == pow2_div(pow2(L), m);
         requires k == ki * m.full;
-        requires 1 <= s < L;
-        requires index == k + j + m.full / 2;
         requires ki < step_count.full;
-        ensures index < N;
+        ensures k + j + m.full / 2 < N;
     {
         pow2_basics(m);
         var half_step := m.full / 2;
 
         calc {
-            index;
+            k + j + m.full / 2;
         ==
             ki * m.full + j + half_step;
         <
@@ -431,16 +43,63 @@ module ntt {
         }
     }
 
-    method ntt_loop_1(a: seq<elem>, s: nat,
+    lemma ntt_chunk_base_case(a': seq<elem>, 
+        k: nat, ki: nat, t: elem, u: elem,
+        m: pow2_t, step_count: pow2_t)
+
+        requires |a'| == N == pow2(L).full;
+        requires m.exp == 1;
+        // requires step_count == pow2_div(pow2(L), m);
+        // requires k == ki * m.full;
+        // requires ki < step_count.full;
+        requires k < k + 1 < N;
+    
+        requires t == modmul(1, Ar()[k + 1]);
+        requires u == Ar()[k];
+        requires a'[k] == modadd(u, t);
+        requires a'[k+1] == modsub(u, t);
+        // ensures 
+    {
+        calc == {
+            t;
+            modmul(1, Ar()[k + 1]);
+            (Ar()[k + 1]) % Q;
+            {
+                assume false;
+            }
+            Ar()[k + 1];
+        }
+
+        var len := pow2(0);
+        pow2_basics(len);
+
+        var even := Ar()[k..k+1];
+        var odd := Ar()[k+1..k+2];
+
+        ntt_rec_base_case(odd, len);
+        ntt_rec_base_case(even, len);
+
+        assert t == poly_eval(odd, omega_nk(len, 0));
+        assert u == poly_eval(even, omega_nk(len, 0));
+
+        var omg := omega_nk(len, 0);
+
+        y_k_value(even + odd, even, odd, pow2(0), pow2(1),
+                omg, k,
+                y_e_k: elem, y_o_k: elem, y_k: elem)
+    }
+
+    method ntt_chunk_loop(a: seq<elem>,
         k: nat, ki: nat,
         m: pow2_t, step_count: pow2_t)
     returns (a': seq<elem>)
+        // combine two chunks into one
         requires |a| == N == pow2(L).full;
         requires 1 <= m.exp <= L;
         requires step_count == pow2_div(pow2(L), m);
         requires k == ki * m.full;
-        requires 1 <= s < L;
         requires ki < step_count.full;
+        requires m.exp == 1 ==> a == Ar();
     {
         a' := a;
         var half_step := m.full / 2;
@@ -453,13 +112,21 @@ module ntt {
             LemmaPow0Auto();
         }
 
+        pow2_basics(m);
+
+        index_bounded_lemma(0, k, ki, m, step_count);
+
         while (j < half_step)
             invariant 0 <= j <= half_step;
             invariant omg == modpow(omgm, j);
             invariant |a'| == |a|;
+            invariant k + j + half_step <= N;
+            invariant a[..k] == a'[..k];
+            invariant a[k+j..k+half_step] == a'[k+j..k+half_step];
+            invariant a[k+half_step+j..] == a'[k+half_step+j..];
+
         {
-            var index := k + j + half_step;
-            index_bounded_lemma(index, j, s, k, ki, m, step_count);
+            index_bounded_lemma(j, k, ki, m, step_count);
             var t := modmul(omg, a[k + j + half_step]);
             var u := a[k + j];
             a' := a'[k + j := modadd(u, t)];
@@ -467,65 +134,85 @@ module ntt {
 
             omg_inv(omgm, omg, m, j);
             omg := modmul(omg, omgm);
+
+            if half_step == 1 {
+                ntt_chunk_base_case(a', k, ki, t, u, m, step_count);
+            }
+
             j := j + 1;
         }
+
+        assert a[..k] == a'[..k];
+        assert a[k+m.full..] == a'[k+m.full..];
+
+        // if m.exp == 1 {
+        //     j := 0;
+        //     index_bounded_lemma(j, s, k, ki, m, step_count);
+
+        //     var t := modmul(omg, a[k + j + half_step]);
+        //     var u := a[k + j];
+
+        //     assert half_step == 1;
+        //     assert a'[k + j] == modadd(u, t);
+
+        // }
     }
 
-    method ntt_loop_0(a: seq<elem>, s: nat)
-        requires |a| == N == pow2(L).full;
-        requires 1 <= s < L;
-    {
-        var m := pow2(s);
-        pow2_basics(m);
-        assume 1 <= m.full <= N/2;
+    // method ntt_level_loop(a: seq<elem>, s: nat)
+    //     requires |a| == N == pow2(L).full;
+    //     requires 1 <= s < L;
+    // {
+    //     var m := pow2(s);
+    //     pow2_basics(m);
+    //     assume 1 <= m.full <= N/2;
 
-        var omgm := omega_nk(m, 1);
+    //     var omgm := omega_nk(m, 1);
 
-        assert omega_nk(m, 1) == omega_n(m) by {
-            LemmaPow1Auto();
-        }
-        var step_size := m.full;
+    //     assert omega_nk(m, 1) == omega_n(m) by {
+    //         LemmaPow1Auto();
+    //     }
+    //     var step_size := m.full;
 
-        var step_count := pow2_div(pow2(L), m);
-        // assert step_count.exp == L - m.exp;
+    //     var step_count := pow2_div(pow2(L), m);
+    //     // assert step_count.exp == L - m.exp;
     
-        var k := 0;
-        var ki := 0;
+    //     var k := 0;
+    //     var ki := 0;
 
-        while (ki < step_count.full)
-            // invariant step_count == pow2_div(pow2(L), m);
-            // invariant step_count.exp == L - m.exp;
-            invariant 0 <= k == ki * step_size;
-        {
-            var k' := k + step_size;
-            var ki' := ki + 1;
+    //     while (ki < step_count.full) // at level s, each chunck is 2 ** s big
+    //         // invariant step_count == pow2_div(pow2(L), m);
+    //         // invariant step_count.exp == L - m.exp;
+    //         invariant 0 <= k == ki * step_size;
+    //     {
+    //         var k' := k + step_size;
+    //         var ki' := ki + 1;
 
-            var _ := ntt_loop_1(a, s, k, ki, m, step_count);
+    //         var _ := ntt_chunk_loop(a, k, ki, m, step_count);
 
-            assert k' == (ki + 1) * step_size by {
-                LemmaMulIsDistributiveAddOtherWay(step_size, ki, 1);
-                assert (ki + 1) * step_size == ki * step_size + 1 * step_size;
-            }
-            assert (ki + 1) * step_size > 0 by {
-                LemmaMulStrictlyPositiveAuto();
-            }
-            k, ki := k', ki';
-        }
-    }
+    //         assert k' == (ki + 1) * step_size by {
+    //             LemmaMulIsDistributiveAddOtherWay(step_size, ki, 1);
+    //             assert (ki + 1) * step_size == ki * step_size + 1 * step_size;
+    //         }
+    //         assert (ki + 1) * step_size > 0 by {
+    //             LemmaMulStrictlyPositiveAuto();
+    //         }
+    //         k, ki := k', ki';
+    //     }
+    // }
 
-    method ntt(b: seq<elem>, len: pow2_t) returns (y: seq<elem>)
-        requires |b | == len.full == N;
-        requires len.exp == L;
-        // ensures poly_eval_all_points(a, y, len)
-    {
-        // var s := pow2(0);
-        var s := 1;
-        while (s < L)
-            invariant 1 <= s;
-        {
-            ntt_loop_0(b, s);
-            s := s + 1;
-        }
-    }
+    // method ntt(b: seq<elem>, len: pow2_t) returns (y: seq<elem>)
+    //     requires |b | == len.full == N;
+    //     requires len.exp == L;
+    //     // ensures poly_eval_all_points(a, y, len)
+    // {
+    //     // var s := pow2(0);
+    //     var s := 1;
+    //     while (s < L) // L levels totoal, combine results at each level 
+    //         invariant 1 <= s;
+    //     {
+    //         ntt_level_loop(b, s);
+    //         s := s + 1;
+    //     }
+    // }
 }
 
