crypto_examples/index.dfy
@@ -1,0 +1,36 @@
+include "omega.dfy"
+include "../std_lib/src/Collections/Sequences/LittleEndianNat.dfy"
+
+module bin refines LittleEndianNat {
+    function method BASE(): nat
+    {
+        2
+    }
+}
+
+module rindex {
+    import opened Power
+
+    import opened omegas
+    import opened pows_of_2
+    import opened bin
+
+    type uint1   =  i: nat | i < 2
+
+    datatype index_raw = index_cons(v: nat, bin: seq<uint1>)
+
+    predicate valid_index(idx: index_raw)
+    {
+        && idx.v < N == Pow(2, L)
+        && idx.bin == FromNatWithLen(idx.v, L)
+    }
+
+    type index_t =  i: index_raw | valid_index(i) witness *
+
+    function method build_index(v: nat): index_t
+        requires v < N
+    {
+        nth_root_lemma();
+        index_cons(v, FromNatWithLen(v, L))
+    }
+}
