crypto_examples/ntt_rec.dfy
@@ -1,0 +1,413 @@
+include "pow2.dfy"
+include "omega.dfy"
+
+module ntt_rec {
+    import opened Seq
+    import opened Power
+    import opened DivMod
+    import opened Mul
+    import opened pows_of_2
+    import opened omegas
+
+    function A(): seq<elem>
+        ensures |A()| == N == pow2(L).full;
+
+    function Ar(): seq<elem>
+        ensures |Ar()| == N == pow2(L).full;
+
+    function {:opaque} poly_eval(a: seq<elem>, x: elem): elem
+    {
+        if |a| == 0 then 0
+        else modadd(First(a), modmul(poly_eval(DropFirst(a), x), x))
+    }
+
+    function method odd_indexed_terms(a: seq<elem>, len: pow2_t): seq<elem>
+        requires |a| == len.full * 2;
+    {
+        seq(len.full, n requires 0 <= n < len.full => a[n * 2 + 1])
+    }
+
+    function method even_indexed_terms(a: seq<elem>, len: pow2_t): seq<elem>
+        requires |a| == len.full * 2;
+    {
+        seq(len.full, n requires 0 <= n < len.full => a[n * 2])
+    }
+
+    lemma poly_eval_base_lemma(a: seq<elem>, x: elem)
+        requires |a| == 1;
+        ensures poly_eval(a, x) == a[0];
+    {
+        reveal poly_eval();
+    }
+
+    lemma {:axiom} poly_eval_split_lemma(a: seq<elem>, 
+        a_e: seq<elem>, a_o: seq<elem>, len: pow2_t, x: elem)
+        requires |a| == len.full * 2;
+        requires a_e == even_indexed_terms(a, len)
+        requires a_o == odd_indexed_terms(a, len)
+        ensures var sqr := modmul(x, x);
+            poly_eval(a, x)
+                == 
+            modadd(poly_eval(a_e, sqr), modmul(x, poly_eval(a_o, sqr)));
+        decreases |a|;
+    {
+        // pow2_basics(len);
+
+        // if |a| == 2 {
+        //     assert a_e == [a[0]];
+        //     assert a_o == [a[1]];
+
+        //     var sqr := modmul(x, x);
+
+        //     calc == {
+        //         poly_eval(a, x);
+        //         {
+        //             reveal poly_eval();
+        //             assert DropFirst(a) == a_o;
+        //         }
+        //         modadd(a[0], modmul(poly_eval(a_o, x), x));
+        //         {
+        //             poly_eval_base_lemma(a_o, x);
+        //             assert poly_eval(a_o, x) == a[1];
+        //         }
+        //         modadd(a[0], modmul(a[1], x));
+        //         {
+        //             poly_eval_base_lemma(a_e, sqr);
+        //             assert poly_eval(a_e, sqr) == a[0];
+        //         }
+        //         modadd(poly_eval(a_e, sqr), modmul(a[1], x));
+        //         {
+        //             poly_eval_base_lemma(a_o, sqr);
+        //             assert poly_eval(a_o, sqr) == a[1];
+        //         }
+        //         modadd(poly_eval(a_e, sqr), modmul(x, poly_eval(a_o, sqr)));
+        //     }
+        //     return;
+        // }
+
+        // var len' := pow2_half(len);
+        // var a_ee := even_indexed_terms(a_e, len');
+        // var a_eo := odd_indexed_terms(a_e, len');
+        // var a_oe := even_indexed_terms(a_o, len');
+        // var a_oo := odd_indexed_terms(a_o, len');
+
+        // calc == {
+        //     poly_eval(a, x);
+        //     {
+        //         reveal poly_eval();
+        //         assert DropFirst(a) == a_o;
+        //     }
+        //     modadd(a[0], modmul(poly_eval(a_o, x), x));
+        // }
+        assume false;
+    }
+
+    predicate poly_eval_all_points(a: seq<elem>, y: seq<elem>, len: pow2_t)
+        requires 0 <= len.exp <= L
+    {
+        && |y| == |a| == len.full
+        && (forall i: nat :: i < len.full ==>
+            y[i] == poly_eval(a, omega_nk(len, i)))
+    }
+
+    lemma y_k_value(a: seq<elem>,
+        a_e: seq<elem>, a_o: seq<elem>,
+        len': pow2_t, len: pow2_t,
+        omg: elem, k: nat,
+        y_e_k: elem, y_o_k: elem, y_k: elem)
+
+        requires |a| == len'.full * 2;
+        requires 1 <= len.exp <= L;
+        requires len'.exp <= L 
+        requires len' == pow2_half(len);
+        requires k < len'.full;
+        requires a_e == even_indexed_terms(a, len');
+        requires a_o == odd_indexed_terms(a, len');
+
+        requires omg == modpow(omega_n(len), k);
+        requires y_e_k == poly_eval(a_e, omega_nk(len', k));
+        requires y_o_k == poly_eval(a_o, omega_nk(len', k));
+        requires y_k == modadd(y_e_k, modmul(omg, y_o_k));
+        
+        ensures y_k == poly_eval(a, omega_nk(len, k));
+    {
+        var x := omega_nk(len, k);
+        var sqr := modmul(x, x);
+
+        calc == {
+            sqr;
+            {
+                omega_nk_square(len, k);
+            }
+            omega_nk(len, 2 * k);
+            {
+                ntt_cancellation_lemma(len, k);
+            }
+            omega_nk(len', k);
+        }
+
+        calc == {
+            poly_eval(a, x);
+            {
+                poly_eval_split_lemma(a, a_e, a_o, len', x);
+            }
+            modadd(poly_eval(a_e, sqr), modmul(x, poly_eval(a_o, sqr)));
+            {
+                assert poly_eval(a_e, sqr) == y_e_k;
+                assert poly_eval(a_o, sqr) == y_o_k;
+            }
+            modadd(y_e_k, modmul(x, y_o_k));
+            y_k;
+        }
+    }
+
+    lemma y_k'_value(a: seq<elem>,
+        a_e: seq<elem>, a_o: seq<elem>,
+        len': pow2_t, len: pow2_t,
+        omg: elem, k: nat,
+        y_e_k: elem, y_o_k: elem, y_k': elem)
+
+        requires |a| == len'.full * 2;
+        requires 1 <= len.exp <= L;
+        requires len'.exp <= L 
+        requires len' == pow2_half(len);
+        requires k < len'.full;
+        requires a_e == even_indexed_terms(a, len');
+        requires a_o == odd_indexed_terms(a, len');
+
+        requires omg == omega_nk(len, k);
+        requires y_e_k == poly_eval(a_e, omega_nk(len', k));
+        requires y_o_k == poly_eval(a_o, omega_nk(len', k));
+        requires y_k' == modsub(y_e_k, modmul(omg, y_o_k));
+
+        ensures y_k' == poly_eval(a, omega_nk(len, k + len'.full));
+    {
+        var x := omega_nk(len, k + len'.full);
+        var sqr := modmul(x, x);
+
+        calc == {
+            sqr;
+            {
+                omega_nk_square(len, k + len'.full);
+            }
+            omega_nk(len, 2 * k + len.full);
+            {
+                ntt_halving_lemma(len, k);
+            }
+            omega_nk(len, 2 * k);
+            {
+                ntt_cancellation_lemma(len, k);
+            }
+            omega_nk(len', k);
+        }
+
+        calc {
+            x;
+            omega_nk(len, k + len'.full);
+            {
+                omega_nk_mul_lemma(len, k, len'.full);
+            }
+            modmul(omg, omega_nk(len, len'.full));
+            {
+                ntt_neg_one_lemma(len);
+            }
+            modmul(omg, Q - 1);
+            (omg * (Q - 1)) % Q;
+            {
+                LemmaMulIsDistributiveSubAuto();
+            }
+            (omg * Q - omg) % Q;
+            {
+                LemmaModMultiplesVanishAuto();
+            }
+            (- (omg as int)) % Q;
+        }
+
+        calc == {
+            poly_eval(a, x);
+            {
+                poly_eval_split_lemma(a, a_e, a_o, len', x);
+            }
+            modadd(poly_eval(a_e, sqr), modmul(x, poly_eval(a_o, sqr)));
+            {
+                assert poly_eval(a_e, sqr) == y_e_k;
+                assert poly_eval(a_o, sqr) == y_o_k;
+            }
+            modadd(y_e_k, modmul(x, y_o_k));
+            (y_e_k + (x * y_o_k) % Q) % Q;
+            {
+                LemmaAddModNoopRight(y_e_k, x * y_o_k, Q);
+            }
+            (y_e_k + x * y_o_k) % Q;
+            (y_e_k + (- (omg as int) % Q) * y_o_k ) % Q;
+            (y_e_k + (- (omg as int) % Q) * (y_o_k % Q)) % Q;
+            {
+                LemmaMulModNoopLeft(- (omg as int), y_o_k, Q);
+            }
+            (y_e_k + ((-(omg as int) * y_o_k) % Q)) % Q;
+            {
+                LemmaAddModNoopRight(y_e_k, -(omg as int) * y_o_k, Q);
+            }
+            (y_e_k + (-(omg as int) * y_o_k)) % Q;
+            (y_e_k + ((-1 * (omg as int)) * y_o_k)) % Q;
+            {
+                LemmaMulIsAssociativeAuto();
+            }
+            (y_e_k - 1 * (omg as int) * y_o_k) % Q;
+            {
+                LemmaMulBasicsAuto();
+            }
+            (y_e_k - (omg as int) * y_o_k) % Q;
+            (y_e_k - (omg * y_o_k)) % Q;
+            {
+                LemmaSubModNoopRight(y_e_k, omg * y_o_k, Q);
+            }
+            (y_e_k - (omg * y_o_k) % Q) % Q;
+            modsub(y_e_k, modmul(omg, y_o_k));
+            y_k';
+        }
+    }
+
+    lemma omg_inv(omgn: elem, omg: elem, len: pow2_t, k: nat)
+        requires len.exp <= L
+        requires omgn == omega_n(len);
+        requires omg == modpow(omgn, k);
+        ensures modmul(omg, omgn) == modpow(omgn, k+1);
+    {
+        var omg' := modmul(omg, omgn);
+        calc == {
+            omg';
+            modmul(omg, omgn);
+            modmul(modpow(omgn, k), omgn);
+            (Pow(omgn, k) % Q * omgn) % Q;
+            {
+                LemmaMulModNoopLeft(Pow(omgn, k), omgn, Q);
+            }
+            (Pow(omgn, k) * omgn) % Q;
+            {
+                LemmaPow1(omgn);
+                assert omgn == Pow(omgn, 1);
+                LemmaPowAdds(omgn, k, 1);
+            }
+            Pow(omgn, k+1) % Q;
+            modpow(omgn, k+1);
+        }
+    }
+
+    lemma ntt_rec_base_case(a: seq<elem>, len: pow2_t)
+        requires len.full == 1;
+        requires |a| == len.full;
+        ensures len.exp == 0;
+        ensures a[0] == poly_eval(a, omega_nk(len, 0));
+    {
+        pow2_basics(len);
+        assert len.exp == 0;
+
+        calc {
+            poly_eval(a, omega_nk(len, 0));
+            {
+                omega_nk_canonical(len, 0);
+                assert omega_nk(len, 0) == 
+                    Pow(G, Pow2(L - len.exp) * 0) % Q;
+            }
+            poly_eval(a, Pow(G, Pow2(L - len.exp) * 0) % Q);
+            poly_eval(a, Pow(G, 0) % Q);
+            {
+                LemmaPow0(G);
+            }
+            poly_eval(a, 1);
+            {
+                poly_eval_base_lemma(a, 1);
+            }
+            a[0];
+        }
+
+    }
+
+    method ntt_rec(a: seq<elem>, len: pow2_t) returns (y: seq<elem>)
+        requires len.exp == L ==> a == A();
+        requires 1 <= len.full;
+        requires len.exp <= L;
+        requires |a| == len.full;
+        ensures poly_eval_all_points(a, y, len)
+        decreases len.full
+    {
+        if len.full == 1 {
+            ntt_rec_base_case(a, len);
+            return a;
+        }
+
+        var len' := pow2_half(len);
+        var a_e := even_indexed_terms(a, len');
+        var a_o := odd_indexed_terms(a, len');
+
+        var y_e := ntt_rec(a_e, len');
+        var y_o := ntt_rec(a_o, len');
+
+        y := seq(len.full, n requires 0 <= n < len.full => 0);
+
+        var omgn := omega_n(len);
+        var omg := 1;
+        var k := 0;
+
+        assert omg == modpow(omgn, 0) by {
+            LemmaPow0Auto();
+        }
+
+        while (k < len'.full)
+            invariant k <= len'.full;
+            invariant |y| == len.full;
+            invariant len.full == len'.full * 2;
+
+            invariant omg == modpow(omgn, k);
+            invariant forall i: nat :: i < k ==> (
+                && y[i] == poly_eval(a, omega_nk(len, i))
+                && y[i + len'.full] == poly_eval(a, omega_nk(len, i + len'.full)))
+            
+            decreases len'.full - k;
+        {
+            var y_e_k := y_e[k];
+            var y_o_k := y_o[k];
+
+            assert y_e_k == poly_eval(a_e, omega_nk(len', k));
+            assert y_o_k == poly_eval(a_o, omega_nk(len', k));
+
+            var y_k := modadd(y_e_k, modmul(omg, y_o_k));
+            y := y[k := y_k];
+
+            var y_k' := modsub(y_e_k, modmul(omg, y_o_k));
+            y := y[k + len'.full := y_k'];
+
+            y_k_value(a, a_e, a_o, len', len, 
+                omg, k, y_e_k, y_o_k, y_k);
+
+            y_k'_value(a, a_e, a_o, len', len, 
+                omg, k, y_e_k, y_o_k, y_k');
+
+            omg_inv(omgn, omg, len, k);
+            omg := modmul(omg, omgn);
+
+            // if len'.full == 1 {
+            //     var i := 0;
+            //     assert k == 0;
+            //     assert y[i] == poly_eval(a, omega_nk(len, i));
+            //     assert y[i + len'.full] == poly_eval(a, omega_nk(len, i + 1));
+            // }
+        
+            k := k + 1;
+        }
+
+        forall i: nat
+            ensures i < len.full ==> y[i] == poly_eval(a, omega_nk(len, i))
+        {
+            if i < len'.full {
+                assert y[i] == poly_eval(a, omega_nk(len, i));
+            } else if i < len.full {
+                var j := i - len'.full;
+                assert y[j + len'.full] ==
+                    poly_eval(a, omega_nk(len, j + len'.full));
+            }
+        }
+    }
+}
+
